Half way through end2end proof for incr

firmware/IncrementWait/CavaIncrementDevice.v
@@ -13,633 +13,23 @@ Require Import Cava.Util.BitArithmetic.
 Require Import Cava.Util.List.
 Require Import Cava.Util.Tactics.
 
+Require Import coqutil.Map.Interface coqutil.Map.Properties.
 Require Import coqutil.Tactics.Simp.
 Require Import coqutil.Tactics.Tactics.
-
-Import ListNotations.
-
-Section Var.
-  Import Expr.
-  Import ExprNotations.
-  Import PrimitiveNotations.
-
-  Local Open Scope N.
-
-  Context {var : tvar}.
-
-  Definition incr_state := BitVec 2.
-  Definition Idle       := Constant incr_state 0.
-  Definition Busy1      := Constant incr_state 1.
-  Definition Busy2      := Constant incr_state 2.
-  Definition Done       := Constant incr_state 3.
-
-  Definition inner
-    : Circuit _ [Bit; BitVec 32] (Bit ** BitVec 32)
-    := {{
-      fun valid data =>
-        let/delay '(istate; value) :=
-           let istate' :=
-               if istate == `Busy1` then `Busy2`
-               else if istate == `Busy2` then `Done`
-                    else if istate == `Done` then `Idle`
-                         else (* istate == `Idle` *)
-                           if valid then `Busy1`
-                           else `Idle` in
-
-           let value' :=
-               if istate == `Busy2` then value + `K 1`
-               else if istate == `Idle` then data
-                    else value in
-
-           (istate', value')
-             initially default
-           : denote_type (incr_state ** BitVec 32)
-        in
-        (istate == `Done`, value)
-       }}.
-
-  Definition incr
-    : Circuit _ [tl_h2d_t] tl_d2h_t
-    := {{
-      fun tl_h2d =>
-        (* Destruct and reassemble tl_h2d with a_address that matches the
-           tlul_adapter_reg interface. *)
-        let '(a_valid
-              , a_opcode
-              , a_param
-              , a_size
-              , a_source
-              , a_address
-              , a_mask
-              , a_data
-              , a_user
-              ; d_ready) := tl_h2d in
-        (* Bit #2 of the address determines which register is being accessed *)
-        (*    (STATUS or VALUE). Zero out the other bits. *)
-        let a_address := a_address & (`K 1` << 2) in
-        let tl_h2d := (a_valid
-                       , a_opcode
-                       , a_param
-                       , a_size
-                       , a_source
-                       , a_address
-                       , a_mask
-                       , a_data
-                       , a_user
-                       , d_ready) in
-
-        let/delay '(busy, done, registers; tl_d2h) :=
-           let '(tl_d2h'; req) := `tlul_adapter_reg` tl_h2d registers in
-           let '(is_read, is_write, address, write_data; _write_mask) := req in
-
-           let '(inner_res_valid; inner_res) := `inner` (!busy && !done && is_write) write_data in
-
-           let busy' :=
-               if busy then !inner_res_valid
-               else !done && is_write in
-
-           let done' :=
-               if busy then inner_res_valid
-               else if done then !(is_read && address == `K 0`)
-                    else done in
-
-           let registers' :=
-               if inner_res_valid then `replace` registers `K (sz:=1) 0` inner_res
-               else registers in
-
-           let registers' :=
-               if busy' then `replace` registers' `K (sz:=1) 1` `K 2`
-               else if done' then `replace` registers' `K (sz:=1) 1` `K 4`
-                    else `replace` registers' `K (sz:=1) 1` `K 1` in
-
-           (busy', done', registers', tl_d2h') initially default
-           : denote_type (Bit ** Bit ** Vec (BitVec 32) 2 ** tl_d2h_t)
-        in
-
-        tl_d2h
-       }}.
-End Var.
-
-Definition sim {s i o} (c : Circuit s i o) (input : list (denote_type i))
-  : list (denote_type s * denote_type i * denote_type o) :=
-  fst (List.fold_left (fun '(acc, s) i =>
-                         let '(s', o) := step c s i in
-                         (acc ++ [(s, i, o)], s'))
-                      input
-                      ([], reset_state c)).
-
-Example sample_trace :=
-  Eval compute in
-    let nop := set_d_ready true tl_h2d_default in
-    let read_reg (r : N) :=
-        set_a_valid true
-        (set_a_opcode Get
-        (set_a_size 2%N
-        (set_a_address r
-        (set_d_ready true tl_h2d_default)))) in
-    let write_val (v : N) :=
-        set_a_valid true
-        (set_a_opcode PutFullData
-        (set_a_size 2%N
-        (set_a_address 0%N (* value-ref *)
-        (set_a_data v
-        (set_d_ready true tl_h2d_default))))) in
-
-    sim incr
-        [ (nop, tt)
-          ; (read_reg 4, tt) (* status *)
-          ; (nop, tt)
-          ; (write_val 42, tt)
-          ; (nop, tt)
-          ; (nop, tt)
-          ; (read_reg 4, tt) (* status *)
-          ; (nop, tt)
-          ; (read_reg 0, tt) (* value *)
-          ; (nop, tt)
-          ; (read_reg 4, tt) (* status *)
-        ]%N.
-(* Print sample_trace. *)
-
-Section Spec.
-  Local Open Scope N.
-
-  Variant inner_state :=
-  | IISIdle
-  | IISBusy (data : N) (count : nat)
-  | IISDone (res : N).
-
-  Notation inner_repr := inner_state.
-
-  Global Instance inner_invariant : invariant_for inner inner_repr :=
-    fun (state : denote_type (state_of inner)) repr =>
-      let '(istate, value) := state in
-      match repr with
-      | IISIdle => istate = 0
-      | IISBusy data c => (0 < c <= 2)%nat /\ istate = N.of_nat c /\ value = data
-      | IISDone res => istate = 3 /\ value = res
-      end.
-
-  Definition inner_spec_step (input : denote_type (input_of inner)) repr :=
-    let '(valid, (data, tt)) := input in
-    match repr with
-    | IISIdle => if valid then IISBusy data 1 else IISIdle
-    | IISBusy data 2 => IISDone ((data + 1) mod 2^32)
-    | IISBusy data c => IISBusy data (c + 1)
-    | IISDone _ => IISIdle
-    end.
-
-  Instance inner_specification
-    : specification_for inner inner_repr :=
-    {| reset_repr := IISIdle;
-
-       update_repr :=
-         fun (input : denote_type (input_of inner)) repr =>
-           inner_spec_step input repr;
-
-       precondition :=
-         fun (input : denote_type (input_of inner)) repr => True;
-
-       postcondition :=
-         fun (input : denote_type (input_of inner)) repr
-           (output : denote_type (output_of inner)) =>
-           let repr' := inner_spec_step input repr in
-           match repr' with
-           | IISDone res => output = (true, res)
-           | _ => exists res, output = (false, res)
-           end;
-    |}.
-
-  Lemma inner_invariant_at_reset : invariant_at_reset inner.
-  Proof.
-    simplify_invariant inner. reflexivity.
-  Qed.
-
-  Lemma inner_invariant_preserved : invariant_preserved inner.
-  Proof.
-    intros (valid, (data, t)) state repr. destruct t.
-    cbn in * |-. destruct state as (istate, value).
-    intros repr' ? Hinvar Hprec; subst.
-    simplify_invariant inner.
-    simplify_spec inner.
-    cbv [inner inner_spec_step]. stepsimpl.
-    repeat (destruct_pair_let; cbn [fst snd]).
-    destruct repr as [|? iiscount|?]; logical_simplify; subst.
-    - destruct valid; cbn; try ssplit; lia.
-    - destruct iiscount as [|[|[|iiscount]]]; cbn; ssplit; lia.
-    - reflexivity.
-  Qed.
-
-  Lemma inner_output_correct : output_correct inner.
-  Proof.
-    intros (valid, (data, t)) state repr. destruct t.
-    cbn in * |-. destruct state as (istate, value).
-    remember (update_repr (c:=inner) (valid, (data, tt)) repr) as repr'.
-    intros Hinvar Hprec.
-    simplify_invariant inner.
-    simplify_spec inner.
-    cbv [inner inner_spec_step]. stepsimpl.
-    repeat (destruct_pair_let; cbn [fst snd]).
-    destruct repr as [|? iiscount|?]; logical_simplify; subst.
-    - destruct valid; eexists; cbn; try ssplit; reflexivity.
-    - destruct iiscount as [|[|[|iiscount]]]; try lia; try eexists; reflexivity.
-    - eexists. reflexivity.
-  Qed.
-
-  Existing Instances inner_invariant_at_reset inner_invariant_preserved
-           inner_output_correct.
-  Global Instance inner_correctness : correctness_for inner.
-  Proof. constructor; typeclasses eauto. Defined.
-
-
-  Variant repr_state :=
-  | RSIdle
-  | RSBusy (data : N)
-  | RSDone (res : N).
-
-  Notation repr := (repr_state * list N * list tl_h2d * inner_repr)%type.
-
-  Global Instance incr_invariant : invariant_for incr repr :=
-    fun (state : denote_type (state_of incr)) repr =>
-      let '((s_busy, (s_done, (s_regs, s_d2h))), (s_tlul, s_inner)) := state in
-      let '(r_state, r_regs, r_tlul, r_inner) := repr in
-      tlul_invariant (reg_count:=2) s_tlul r_tlul
-      /\ inner_invariant s_inner r_inner
-      /\ match r_state with
-        | RSIdle => s_busy = false /\ s_done = false
-                   /\ r_inner = IISIdle
-        | RSBusy data => s_busy = true /\ s_done = false
-                        /\ exists c, r_inner = IISBusy data c
-        | RSDone res => s_busy = false /\ s_done = true
-                       /\ (r_inner = IISDone res \/ r_inner = IISIdle)
-        end
-      /\ s_regs = r_regs.
-
-  Existing Instance tlul_specification.
-
-  Instance incr_specification
-    : specification_for incr repr :=
-    {| reset_repr := (RSIdle, [0; 0], [], IISIdle);
-
-       update_repr :=
-         fun (input : denote_type (input_of incr)) repr =>
-           let '(i_h2d, tt) := input in
-           let '(r_state, r_regs, r_tlul, r_inner) := repr in
-
-           let h2d := set_a_address (N.land (a_address i_h2d) 4) i_h2d in
-
-           let r_tlul' :=
-               let tlul_input := (h2d, (r_regs, tt)) in
-               update_repr (c:=tlul_adapter_reg (reg_count:=2))
-                           tlul_input r_tlul in
-
-           (* compute (some) tlul output *)
-           let '(is_read, is_write, address, write_data) :=
-               match outstanding_h2d (h2d :: r_tlul) with
-               | None => (false, false, 0, 0)
-               | Some h2d' =>
-                 if a_opcode h2d' =? Get then
-                   match outstanding_h2d r_tlul with
-                   | None => (a_valid h2d, false, a_address h2d, 0)
-                   | _ => (false, false, 0, 0)
-                   end
-                 else if a_opcode h2d' =? PutFullData then
-                   match outstanding_h2d r_tlul with
-                   | None => (false, a_valid h2d, a_address h2d, a_data h2d)
-                   | _ => (false, false, 0, 0)
-                   end
-                 else (false, false, 0, 0)
-               end in
-
-           let r_inner' :=
-               let inner_input := (match r_state with RSIdle => is_write | _ => false end, (write_data, tt)) in
-               update_repr (c:=inner) inner_input r_inner in
-
-           let r_state' :=
-               match r_state with
-               | RSDone _ =>
-                 if negb (is_read && (address =? 0)) then r_state
-                 else RSIdle
-               | _ =>
-                 match r_inner' with
-                 | IISBusy data _ => RSBusy data
-                 | IISDone res => RSDone res
-                 | _ => r_state
-                 end
-               end in
-
-           let r_regs' :=
-               match r_inner' with
-               | IISDone res => replace 0 res r_regs
-               | _ => r_regs
-               end in
-
-           let r_regs' :=
-               match r_state' with
-               | RSIdle => replace 1 1 r_regs'
-               | RSBusy _ => replace 1 2 r_regs'
-               | RSDone _ => replace 1 4 r_regs'
-               end in
-
-           (r_state', r_regs', h2d :: r_tlul, r_inner');
-
-       precondition :=
-         fun (input : denote_type (input_of incr)) repr =>
-           let '(i_h2d, tt) := input in
-           let '(r_state, r_regs, r_tlul, r_inner) := repr in
-
-           let h2d := set_a_address (N.land (a_address i_h2d) 4) i_h2d in
-
-           let tlul_input := (h2d, (r_regs, tt)) in
-
-           let prec_tlul :=
-               precondition (tlul_adapter_reg (reg_count:=2))
-                            tlul_input r_tlul in
-
-           let prec_inner :=
-               forall d2h is_read is_write address write_data write_mask,
-                 postcondition (tlul_adapter_reg (reg_count:=2))
-                               tlul_input r_tlul
-                               (d2h, (is_read, (is_write, (address, (write_data, write_mask)))))
-                 -> precondition inner (match r_state with RSIdle => is_write | _ => false end, (write_data, tt)) r_inner in
-
-           prec_tlul /\ prec_inner;
-
-       postcondition :=
-         fun (input : denote_type (input_of incr)) repr
-           (output : denote_type (output_of incr)) =>
-           let '(i_h2d, tt) := input in
-           let '(r_state, r_regs, r_tlul, r_inner) := repr in
-
-           let h2d := set_a_address (N.land (a_address i_h2d) 4) i_h2d in
-
-           let postc_tlul :=
-               let tlul_input := (h2d, (r_regs, tt)) in
-               exists req,
-                 postcondition (tlul_adapter_reg (reg_count:=2))
-                               tlul_input r_tlul
-                               (output, req) in
-           postc_tlul;
-    |}.
-
-  Lemma incr_invariant_at_reset : invariant_at_reset incr.
-  Proof.
-    simplify_invariant incr.
-    cbn. ssplit; try reflexivity.
-    apply (tlul_adapter_reg_invariant_at_reset (reg_count:=2)).
-  Qed.
-
-  Existing Instance tlul_adapter_reg_correctness.
-
-  (* TODO: move these lemmas to TLUL.v *)
-  Lemma outstanding_in_repr {reg_count : nat} : forall r_tlul t,
-      outstanding_h2d r_tlul = Some t ->
-      In t r_tlul.
-  Proof.
-    intros ? ?.
-    induction r_tlul; intros Houts; cbn in Houts.
-    - discriminate.
-    - destruct (outstanding_h2d r_tlul) eqn:Houts'.
-      + destruct d_ready.
-        * discriminate.
-        * apply in_cons. auto.
-      + destruct (a_valid a).
-        * inversion Houts. apply in_eq.
-        * discriminate.
-  Qed.
-
-  Lemma outstanding_a_valid {reg_count : nat} : forall r_tlul t,
-      outstanding_h2d r_tlul = Some t ->
-      a_valid t = true.
-  Proof.
-    intros ? ?.
-    induction r_tlul; intros Houts; cbn in Houts.
-    - discriminate.
-    - destruct (outstanding_h2d r_tlul) eqn:Houts'.
-      + destruct d_ready.
-        * discriminate.
-        * auto.
-      + destruct (a_valid a) eqn:Hvalid.
-        * inversion Houts. subst. assumption.
-        * discriminate.
-  Qed.
-
-  Lemma outstanding_prec {reg_count : nat} : forall tl_st r_tlul t,
-      tlul_invariant (reg_count:=reg_count) tl_st r_tlul ->
-      outstanding_h2d r_tlul = Some t ->
-      a_opcode t = Get \/ a_opcode t = PutFullData.
-  Proof.
-    intros ? ? ? Hinvar Houts. simpl in *.
-    apply (outstanding_in_repr (reg_count:=reg_count)) in Houts as Hin.
-    unfold tlul_invariant in Hinvar. logical_simplify.
-    eapply Forall_forall in H. 2: apply Hin.
-    apply H.
-    eapply (outstanding_a_valid (reg_count:=reg_count)).
-    apply Houts.
-  Qed.
-
-
-  Lemma incr_invariant_preserved : invariant_preserved incr.
-  Proof.
-    intros (h2d, t) state (((r_state, r_regs), r_tlul), r_inner). destruct t.
-    cbn in * |-. destruct state as ((busy, (done, (registers, d2h))), (tl_st, inner_st)).
-    destruct_tl_h2d. destruct_tl_d2h.
-    intros repr' ? Hinvar Hprec; subst.
-    simplify_invariant incr. logical_simplify. subst.
-    simplify_spec incr. logical_simplify. subst.
-    (* destruct Hprec as [regs Hprec]. *)
-    cbv [incr]. stepsimpl.
-    use_correctness.
-    match goal with
-    | H: (match outstanding_h2d (_::r_tlul) with | _ => _ end) |- _ =>
-      rename H into Htl_postc
-    end.
-    repeat (destruct_pair_let; cbn [fst snd]).
-    ssplit.
-    - eapply tlul_adapter_reg_invariant_preserved.
-      2: apply H.
-      + reflexivity.
-      + assumption.
-    - eapply inner_invariant_preserved.
-      2: apply H0.
-      + simpl in *.
-        destruct r_inner; try reflexivity.
-        destruct (outstanding_h2d r_tlul) eqn:Houts.
-        * destruct d_ready; logical_simplify; subst.
-          -- boolsimpl. destruct r_state; reflexivity.
-          -- eapply outstanding_prec in H as Hprec_t. 2: apply Houts.
-             destruct Hprec_t as [Hprec_t|Hprec_t];
-               rewrite Hprec_t in *; cbn in Htl_postc |- *; logical_simplify; subst;
-                 boolsimpl; destruct r_state; reflexivity.
-        * destruct a_valid eqn:Hvalid; logical_simplify; subst.
-          -- cbn in Htl_postc.
-             match goal with
-             | H: true = true -> _ |- _ =>
-               destruct H; try reflexivity; subst
-             end; cbn in Htl_postc; logical_simplify; subst;
-               boolsimpl; destruct r_state; logical_simplify; subst;
-                 reflexivity.
-          -- boolsimpl; destruct r_state; reflexivity.
-      + match goal with
-        | H: context [_ -> precondition inner _ r_inner] |- _ =>
-          eapply H
-        end.
-        do 8 eexists. ssplit.
-        1-2: reflexivity.
-        apply Htl_postc.
-    - match goal with
-      | H: context [_ -> precondition inner _ r_inner] |- _ => clear H
-      end.
-      destruct r_inner; destruct r_state; destruct inner_st;
-        unfold inner_invariant in H0; logical_simplify; subst;
-          try discriminate;
-          try (destruct H4; discriminate).
-      all: destruct (outstanding_h2d r_tlul) eqn:Houts;
-        cbn [outstanding_h2d] in Htl_postc |- *; rewrite Houts in Htl_postc |- *.
-      all: tlsimpl; destruct d_ready; logical_simplify; subst; boolsimpl.
-      all: cbn; try (ssplit; reflexivity).
-      all: try (eapply outstanding_prec in H;
-                try match goal with
-                    | H: outstanding_h2d _ = Some _ |- outstanding_h2d _ = Some _ =>
-                      apply H
-                    end; destruct H; rewrite H in Htl_postc |- *; cbn in Htl_postc |- *;
-                logical_simplify; subst; ssplit;
-                try (left; reflexivity);
-                try (right; reflexivity);
-                reflexivity).
-      all: try (destruct a_valid; simplify_spec (tlul_adapter_reg (reg_count:=2));
-                tlsimpl; destruct H2;
-                try match goal with
-                    | H: true = true -> _ |- _ =>
-                      destruct H; try reflexivity; subst
-                    end; cbn in Htl_postc; logical_simplify; subst; cbn; ssplit;
-                  try eexists; reflexivity).
-      all: try (destruct a_valid; ssplit;
-                try (left; reflexivity);
-                try (right; reflexivity);
-                reflexivity).
-      all: try (destruct a_valid; simplify_spec (tlul_adapter_reg (reg_count:=2));
-                tlsimpl; destruct H2;
-                try match goal with
-                    | H: true = true -> _ |- _ =>
-                      destruct H; try reflexivity; subst
-                    end; cbn in Htl_postc; logical_simplify; subst;
-                boolsimpl; destruct (negb (N.land a_address 4 =? 0)) eqn:Haddr;
-                cbn; try (rewrite Haddr); ssplit;
-                try (left; reflexivity);
-                try (right; reflexivity);
-                reflexivity).
-      all: (inversion H4; subst; clear H4;
-            destruct x as [|[|[|?]]]; cbn; ssplit;
-            try eexists;
-            try (left; reflexivity);
-            try (right; reflexivity);
-            try reflexivity;
-            exfalso; lia).
-    - match goal with
-      | H: context [_ -> precondition inner _ r_inner] |- _ => clear H
-      end.
-      destruct r_inner; destruct r_state; destruct inner_st;
-        unfold inner_invariant in H0; logical_simplify; subst;
-          try discriminate.
-      all: destruct (outstanding_h2d r_tlul) eqn:Houts;
-        cbn [outstanding_h2d] in Htl_postc |- *; rewrite Houts in Htl_postc |- *.
-      all: tlsimpl; destruct d_ready; logical_simplify; subst; boolsimpl.
-      all: try reflexivity.
-      all: try (eapply outstanding_prec in H;
-                try match goal with
-                    | H: outstanding_h2d _ = Some _ |- outstanding_h2d _ = Some _ =>
-                      apply H
-                    end; destruct H; rewrite H in Htl_postc |- *; cbn in Htl_postc |- *;
-                logical_simplify; subst; cbn; reflexivity).
-      all: try (destruct a_valid; simplify_spec (tlul_adapter_reg (reg_count:=2));
-                tlsimpl; destruct H2;
-                try match goal with
-                    | H: true = true -> _ |- _ =>
-                      destruct H; try reflexivity; subst
-                    end; cbn in Htl_postc; logical_simplify; subst; reflexivity).
-      all: try (destruct a_valid; simplify_spec (tlul_adapter_reg (reg_count:=2));
-                tlsimpl; destruct H2;
-                try match goal with
-                    | H: true = true -> _ |- _ =>
-                      destruct H; try reflexivity; subst
-                    end; cbn in Htl_postc; logical_simplify; subst;
-                boolsimpl; destruct (negb (N.land a_address 4 =? 0)) eqn:Haddr;
-                cbn; try (rewrite Haddr); reflexivity).
-      all: try (inversion H4; subst; clear H4;
-            destruct x as [|[|[|?]]]; try reflexivity; exfalso; lia).
-      all: try (destruct H4; discriminate).
-  Qed.
-
-  Lemma incr_output_correct : output_correct incr.
-  Proof.
-    intros (h2d, t) state (((r_state, r_regs), r_tlul), r_inner). destruct t.
-    cbn in * |-. destruct state as ((busy, (done, (registers, d2h))), (tl_st, inner_st)).
-    destruct_tl_h2d. destruct_tl_d2h.
-    intros Hinvar Hprec; subst.
-    simplify_invariant incr. logical_simplify. subst.
-    simplify_spec incr. logical_simplify. subst.
-    cbv [incr]. stepsimpl.
-    use_correctness.
-    match goal with
-    | H: (match outstanding_h2d (_::r_tlul) with | _ => _ end) |- _ =>
-      rename H into Htl_postc
-    end.
-    repeat (destruct_pair_let; cbn [fst snd]).
-    tlsimpl.
-    destruct r_inner; destruct r_state; destruct inner_st;
-      unfold inner_invariant in H0; logical_simplify; subst;
-        try discriminate;
-        try (destruct H5; discriminate).
-    all: destruct (outstanding_h2d r_tlul) eqn:Houts;
-      cbn [outstanding_h2d] in Htl_postc |- *; rewrite Houts in Htl_postc |- *.
-    all: tlsimpl; destruct d_ready; logical_simplify; subst; boolsimpl.
-    all: do 9 eexists.
-    all: ssplit; try reflexivity; tlsimpl; ssplit; try reflexivity; try assumption.
-    all: try (eapply outstanding_prec in H;
-              try match goal with
-                  | H: outstanding_h2d _ = Some _ |- outstanding_h2d _ = Some _ =>
-                    apply H
-                  end; destruct H; rewrite H in Htl_postc |- *; cbn in Htl_postc |- *;
-              logical_simplify; subst; ssplit;
-              try (left; reflexivity);
-              try (right; reflexivity);
-              try assumption;
-              reflexivity).
-    all: try (destruct a_valid; simplify_spec (tlul_adapter_reg (reg_count:=2));
-              tlsimpl; destruct H2;
-              try match goal with
-                  | H: true = true -> _ |- _ =>
-                    destruct H; try reflexivity; subst
-                  end; cbn in Htl_postc; logical_simplify; subst; cbn; ssplit;
-              try eexists; try assumption; reflexivity).
-    Unshelve. all: auto.
-  Qed.
-
-  Existing Instances incr_invariant_at_reset incr_invariant_preserved
-           incr_output_correct.
-  Global Instance incr_correctness : correctness_for incr.
-  Proof. constructor; typeclasses eauto. Defined.
-End Spec.
-
-Require Import Coq.micromega.Lia.
+Require Import coqutil.Word.Interface coqutil.Word.Properties.
 
 Require Import riscv.Utility.Utility.
-
-Require Import coqutil.Map.Interface coqutil.Map.Properties.
-Require Import coqutil.Word.Interface coqutil.Word.Properties.
-Require Import coqutil.Tactics.Tactics.
-Require Import coqutil.Tactics.Simp.
-Require Import coqutil.Tactics.fwd.
 
 Require Import bedrock2.ZnWords.
 
 Require Import Bedrock2Experiments.RiscvMachineWithCavaDevice.InternalMMIOMachine.
 Require Import Bedrock2Experiments.IncrementWait.Constants.
+Require Import Bedrock2Experiments.IncrementWait.Incr.
 Require Import Bedrock2Experiments.IncrementWait.IncrementWaitSemantics.
 Require Import Bedrock2Experiments.StateMachineSemantics.
 Require Import Bedrock2Experiments.RiscvMachineWithCavaDevice.MMIOToCava.
 
-Require Import Cava.Util.Tactics.
+Import ListNotations.
 
 Section WithParameters.
   Instance var : tvar := denote_type.
@@ -647,32 +37,10 @@ Section WithParameters.
   Context {word: Interface.word 32} {word_ok: word.ok word}
           {Mem: map.map word byte} {Registers: map.map Z word}.
 
-  Definition consistent_states
-             '((reqid, (reqsz, (rspop, (error, (outstanding, (_we_o, _re_o))))))
-               : denote_type (state_of (tlul_adapter_reg (reg_count := 2))))
-             '((d_valid, (d_opcode, (d_param, (d_size, (d_source, (d_sink, (d_data, (d_user, (d_error, a_ready)))))))))
-               : denote_type tl_d2h_t)
-    : Prop :=
-      d_valid = outstanding /\
-      d_opcode = rspop /\
-      (* d_param = 0 /\ *)
-      d_size = reqsz /\
-      d_source = reqid /\
-      (* d_sink = 0 /\ *)
-      (* d_data = ?? *)
-      (* d_user = 0 /\ *)
-      d_error = error /\
-      a_ready = negb outstanding.
-
-  Definition mk_counter_state (istate : N) (val : N) tl_d2h tlul_state
-    : denote_type (state_of incr) :=
-    ((istate, (val, tl_d2h)), tlul_state).
-
   Global Instance counter_device: device := {|
     device.state := denote_type (state_of incr);
-    device.is_ready_state s := exists val tl_d2h tlul_state,
-        consistent_states tlul_state tl_d2h
-        /\ s = mk_counter_state 0 val tl_d2h tlul_state;
+    device.is_ready_state s := exists r_regs r_tlul r_inner,
+        incr_invariant s (RSIdle, r_regs, r_tlul, r_inner);
     device.run1 s i := Semantics.step incr s (i, tt);
     device.addr_range_start := INCR_BASE_ADDR;
     device.addr_range_pastend := INCR_END_ADDR;
@@ -687,27 +55,26 @@ Section WithParameters.
   Global Instance circuit_spec : circuit_behavior :=
   {| ncycles_processing := 15%nat |}.
 
-  Inductive counter_related: IncrementWaitSemantics.state -> denote_type (state_of incr) -> Prop :=
-  | IDLE_related: forall val tl_d2h tlul_state,
-      consistent_states tlul_state tl_d2h ->
-      counter_related IDLE (mk_counter_state 0 val tl_d2h tlul_state)
-  | BUSY1_related: forall val tl_d2h tlul_state ncycles,
-      (1 < ncycles)%nat ->
-      consistent_states tlul_state tl_d2h ->
-      counter_related (BUSY val ncycles) (mk_counter_state 1 (word_to_N val) tl_d2h tlul_state)
-  | BUSY2_related: forall val tl_d2h tlul_state ncycles,
+  Inductive counter_related_spec: IncrementWaitSemantics.state -> repr -> Prop :=
+  | IDLE_related: forall r_regs r_tl r_inner,
+      counter_related_spec IDLE (RSIdle, r_regs, r_tl, r_inner)
+  | BUSY_related: forall r_regs r_tl r_inner val ncycles,
       (0 < ncycles)%nat ->
-      consistent_states tlul_state tl_d2h ->
-      counter_related (BUSY val ncycles) (mk_counter_state 2 (word_to_N val) tl_d2h tlul_state)
+      counter_related_spec (BUSY val ncycles)
+                           (RSBusy (word_to_N val), r_regs, r_tl, r_inner)
   (* the hardware is already done, but the software hasn't polled it yet to find out,
      so we have to relate a software-BUSY to a hardware-done: *)
-  | BUSY_done_related: forall val tl_d2h tlul_state ncycles,
-      consistent_states tlul_state tl_d2h ->
-      counter_related (BUSY val ncycles)
-                      (mk_counter_state 3 (word_to_N (word.add (word.of_Z 1) val)) tl_d2h tlul_state)
-  | DONE_related: forall val tl_d2h tlul_state,
-      consistent_states tlul_state tl_d2h ->
-      counter_related (DONE val) (mk_counter_state 3 (word_to_N val) tl_d2h tlul_state).
+  | BUSY_done_related: forall r_regs r_tl r_inner val ncycles,
+      counter_related_spec (BUSY val ncycles)
+                           (RSDone (word_to_N (word.add (word.of_Z 1) val)), r_regs, r_tl, r_inner)
+  | DONE_related: forall r_regs r_tl r_inner val,
+      nth 0 r_regs 0%N = (word_to_N val)
+      -> counter_related_spec (DONE val)
+                             (RSDone (word_to_N val), r_regs, r_tl, r_inner).
+
+  Definition counter_related (sH : IncrementWaitSemantics.state)
+             (sL : denote_type (state_of incr)) : Prop :=
+    exists repr, counter_related_spec sH repr /\ incr_invariant sL repr.
 
   (* This should be in bedrock2.ZnWords. It is use by ZnWords, which is used in
      the two following Lemmas. *)
@@ -737,198 +104,365 @@ Section WithParameters.
       eapply pair_equal_spec in H; destruct H as [?H0 ?H1]
     end.
 
-  Ltac destruct_tlul_adapter_reg_state :=
-    match goal with
-    | H : N * (N * (N * (bool * (bool * (bool * bool))))) |- _ =>
-      destruct H as [?reqid [?reqsz [?rspop [?error [?outstanding [?we_o ?re_o]]]]]]
-    end.
-
-  Ltac destruct_consistent_states :=
-    match goal with
-    | H : consistent_states _ _ |- _ =>
-      destruct H as (Hvalid & Hopcode & Hsize & Hsource & Herror & Hready)
-    end.
+  (* Ltac destruct_tlul_adapter_reg_state := *)
+  (*   match goal with *)
+  (*   | H : N * (N * (N * (bool * (bool * (bool * bool))))) |- _ => *)
+  (*     destruct H as [?reqid [?reqsz [?rspop [?error [?outstanding [?we_o ?re_o]]]]]] *)
+  (*   end. *)
 
   Lemma N_to_word_word_to_N: forall v, N_to_word (word_to_N v) = v.
   Proof. intros. unfold N_to_word, word_to_N. ZnWords. Qed.
 
-(* TODO move to coqutil *)
-Ltac contradictory H :=
-  lazymatch type of H with
-  | ?x <> ?x => exfalso; apply (H eq_refl)
-  | False => case H
-  end.
-Require Import coqutil.Tactics.autoforward.
-Ltac fwd_step ::=
-  match goal with
-  | H: ?T |- _ => is_destructible_and T; destr_and H
-  | H: exists y, _ |- _ => let yf := fresh y in destruct H as [yf H]
-  | H: ?x = ?x |- _ => clear H
-  | H: True |- _ => clear H
-  | H: ?LHS = ?RHS |- _ =>
-    let h1 := head_of_app LHS in is_constructor h1;
-    let h2 := head_of_app RHS in is_constructor h2;
-    (* if not eq, H is a contradiction, but we don't want to change the number
-       of open goals in this tactic *)
-    constr_eq h1 h2;
-    (* we don't use `inversion H` or `injection H` because they unfold definitions *)
-    inv_rec LHS RHS;
-    clear H
-  | E: ?x = ?RHS |- context[match ?x with _ => _ end] =>
-    let h := head_of_app RHS in is_constructor h; rewrite E in *
-  | H: context[match ?x with _ => _ end], E: ?x = ?RHS |- _ =>
-    let h := head_of_app RHS in is_constructor h; rewrite E in *
-  | H: context[match ?x with _ => _ end] |- _ =>
-    (* note: recursive invocation of fwd_step for contradictory cases *)
-    destr x; try solve [repeat fwd_step; contradictory H]; []
-  | H: _ |- _ => autoforward with typeclass_instances in H
-  | |- _ => progress subst
-  | |- _ => progress fwd_rewrites
-  end.
+  Existing Instance Incr.inner_specification.
+  Existing Instance Incr.inner_correctness.
+  Existing Instance Incr.inner_invariant.
 
-  Axiom TODO: False.
+  Existing Instance TLUL.tlul_specification.
+  Existing Instance TLUL.tlul_adapter_reg_correctness.
+  Existing Instance TLUL.tlul_invariant.
+
+  Existing Instance incr_specification.
+  Existing Instance incr_correctness.
+
+  Lemma runUntilResp_big_step : forall s h2d repr,
+      precondition incr (h2d, tt) repr
+      -> a_valid h2d = true
+      -> d_ready h2d = true (* TODO: do we need this? *)
+      -> incr_invariant s repr
+      -> exists n inputs s' repr' d2h s'',
+          device.runUntilResp h2d device.maxRespDelay s = (Some d2h, s'')
+          /\ n <= device.maxRespDelay
+          /\ inputs = repeat (h2d, tt) n
+          /\ s' = snd (simulate' incr inputs s)
+          (* /\ (s'', d2h) = Semantics.step incr s' (h2d, tt) *)
+          /\ repr' = fold_left (fun r i => update_repr (c:=incr) i r) inputs repr
+          (* /\ invariant s' repr' *)
+          /\ postcondition incr (h2d, tt) repr' d2h
+          /\ d_valid d2h = true
+          /\ incr_invariant s'' (update_repr (c:=incr) (h2d, tt) repr').
+  Proof.
+    intros ? ? ? Hprec Ea_valid Ed_ready Hinv.
+    unfold device.maxRespDelay, device.runUntilResp, device.state, device.run1, counter_device,
+    state_machine.read_step, increment_wait_state_machine, read_step in *.
+    eapply output_correct_pf in Hinv as Houtput.
+    apply Houtput in Hprec as Hpostc. clear Houtput.
+    cbn in s, h2d. destruct_tl_h2d.
+    destruct repr as (((?r_state, ?r_regs), ?r_tl), ?r_inner).
+    assert (Hprec_temp := Hprec).
+    unfold precondition, incr_specification in Hprec_temp.
+    logical_simplify.
+    unfold precondition, tlul_specification in H.
+    logical_simplify. tlsimpl. subst.
+    unfold postcondition, incr_specification in Hpostc.
+    unfold postcondition, tlul_specification in Hpostc.
+    destruct Hpostc as [[is_read [is_write [address [w_val w_mask]]]] [h2d' [regs' [d2h' [is_read' [is_write' [address' [w_val' [w_mask' Hpostc]]]]]]]]].
+    destruct_tl_h2d. destruct_tl_d2h. tlsimpl.
+    destruct Hpostc as [Hpostc1 [Hpostc2 Hpostc3]].
+    subst.
+    apply pair_equal_spec in Hpostc2.
+    logical_simplify.
+    cbn [outstanding_h2d] in Hpostc3.
+    destruct (outstanding_h2d r_tl) eqn:Eouts.
+    - cbn in Hpostc3. logical_simplify. subst.
+      assert (Hprec':
+                precondition incr
+                             (true,
+                              (a_opcode0,
+                               (a_param0, (a_size0, (a_source0, (a_address, (a_mask0, (a_data0, (a_user0, true)))))))), tt)
+                             (update_repr (c:=incr)
+                                          (true,
+                                           (a_opcode0,
+                                            (a_param0, (a_size0, (a_source0, (a_address, (a_mask0, (a_data0, (a_user0, true)))))))), tt)
+                                          (r_state, regs', r_tl, r_inner))).
+      { simplify_spec incr.
+        cbn [outstanding_h2d]. rewrite Eouts.
+        tlsimpl. ssplit.
+        - simplify_spec (tlul_adapter_reg (reg_count:=2)). tlsimpl. split; [|assumption].
+          match goal with
+          | |- context [length (match ?m with | _=> _ end)] =>
+            destruct m
+          end;
+          match goal with
+          | |- context [replace _ _ (match ?m with | _=> _ end)] =>
+            destruct m
+          end; rewrite ! length_replace; assumption.
+        - simplify_spec Incr.inner. intros. apply I.
+      }
+      destruct H1; [auto|..]; subst.
+      all: exists 1.
+      all: destruct_pair_let;
+        match goal with
+        | |- context [if d_valid ?c then _ else _] =>
+          match type of H2 with
+          | _ = ?r => replace c with r
+          end
+        end.
+      all: tlsimpl;
+        assert (Hinv' := Hprec);
+        eapply incr_invariant_preserved in Hinv;
+        [apply Hinv in Hinv'|reflexivity]; clear Hinv.
+      all: eapply output_correct_pf in Hinv' as Houtput';
+        apply Houtput' in Hprec' as Hpostc'; clear Houtput';
+          assert (Hpostc'' := Hpostc');
+        unfold postcondition, incr_specification in Hpostc';
+        unfold postcondition, tlul_specification in Hpostc';
+        cbn [update_repr outstanding_h2d] in Hpostc';
+        rewrite Eouts in Hpostc'; cbn -[Semantics.step] in Hpostc';
+        destruct Hpostc' as [[is_read [is_write [address [w_val w_mask]]]] [h2d' [regs'' [d2h' [is_read' [is_write' [address'' [w_val'' [w_mask'' Hpostc']]]]]]]]].
+      all: destruct_tl_h2d; destruct_tl_d2h; tlsimpl;
+        destruct Hpostc' as [Hpostc1' [Hpostc2' Hpostc3']];
+        subst;
+        apply pair_equal_spec in Hpostc2';
+        logical_simplify;
+        rewrite Eouts in Hpostc3';
+        tlsimpl.
+      all: cbn in Hpostc3'; logical_simplify; subst.
+      all: do 5 eexists; ssplit; try reflexivity.
+      1,5: destruct_pair_let;
+                match goal with
+        | |- context [if d_valid ?c then _ else _] =>
+          match type of H1 with
+          | _ = ?r => replace c with r
+          end
+        end; tlsimpl; reflexivity.
+      1,4: cbn [repeat fold_left];
+        match goal with
+        | H: postcondition incr _ _ ?c |- _ =>
+          match type of H1 with
+          | _ = ?r => replace c with r in H; apply H
+          end
+        end.
+      1,3: reflexivity.
+      1,2: cbn [repeat fold_left];
+        eapply incr_invariant_preserved; [reflexivity|assumption..].
+    - destruct H1; [auto|..]; subst; cbn in Hpostc3; logical_simplify; subst.
+      all: exists 0.
+      all: do 5 eexists; ssplit; try reflexivity; try lia.
+      1,5: destruct_pair_let;
+        match goal with
+        | |- context [if d_valid ?c then _ else _] =>
+          match type of H2 with
+          | _ = ?r => replace c with r
+          end
+        end; tlsimpl; reflexivity.
+      1,4: cbn [repeat fold_left];
+        eapply output_correct_pf in Hinv as Houtput;
+        apply Houtput in Hprec;
+        match goal with
+        | H: postcondition incr _ _ ?c |- _ =>
+          match type of H2 with
+          | _ = ?r => replace c with r in H; apply H
+          end
+        end.
+      1,3: reflexivity.
+      1,2: cbn [repeat fold_left];
+        eapply incr_invariant_preserved; [reflexivity|assumption..].
+  Qed.
 
   (* Set Printing All. *)
   Global Instance cava_counter_satisfies_state_machine:
     device_implements_state_machine counter_device increment_wait_state_machine.
   Proof.
-    eapply Build_device_implements_state_machine with (device_state_related := counter_related);
-      intros.
+    eapply Build_device_implements_state_machine with (device_state_related := counter_related).
     - (* mmioAddrs_match: *)
       reflexivity.
     - (* initial_state_is_ready_state: *)
-      simpl in *. subst. inversion H0. subst. eexists _, _, _. eauto.
+      intros ? ? Hinit Hrel.
+      cbn in *. subst. destruct Hrel as [?repr [?Hrel ?Hinv]].
+      inversion Hrel. subst.
+      do 3 eexists. eapply Hinv.
     - (* initial_states_are_related: *)
-      simpl in *. destruct H0 as (val & tl_d2h & tlul_state & H0 & H1). subst.
-      eauto using IDLE_related.
+      intros ? ? Hinit Hready.
+      cbn in *. destruct Hready as (?r_regs & ?r_tl & ?r_inner & ?Hinv). subst.
+      unfold counter_related. eexists. split; [|apply Hinv].
+      apply IDLE_related.
     - (* initial_state_exists: *)
-      simpl in *. destruct H as (val & tl_d2h & tlul_state & H0 & H1). subst.
-      eauto using IDLE_related.
+      intros ? Hready.
+      cbn in *. destruct Hready as (?r_regs & ?r_tl & ?r_inner & ?Hinv).
+      eexists. split; [reflexivity|].
+      unfold counter_related. eexists. split; [|apply Hinv].
+      apply IDLE_related.
     - (* nonMMIO_device_step_preserves_state_machine_state: *)
-      simpl in sL1, sL2.
-      destruct_tl_h2d. simpl in H. subst.
-      cbn in H1.
-      repeat (destruct_pair_let_hyp;
-              repeat (destruct_pair_equal_hyp; subst; cbn [fst snd])).
-      inversion H0; subst;
+      intros ? ? ? ? ? Ha_valid Hrel.
+      (* cbn in sL1, sL2. *)
+      (* destruct sL2 as ((?busy, (?done, (?regs, ?d2h))), (?s_tl, ?s_inner)). *)
+      (* destruct_tl_h2d. destruct_tl_d2h. tlsimpl. subst. *)
+      unfold device.run1. unfold counter_device.
+      intros Hstep.
+      destruct Hrel as [?repr [?Hrel ?Hinv]].
+      assert (Hprec: precondition incr (h2d, tt) repr).
+      { destruct_tl_h2d. destruct_tl_d2h. tlsimpl.
+        cbn in sL1; destruct sL1 as ((?busy, (?done, (?regs, ?d2h))), (?s_tl, ?s_inner)).
+        destruct repr as (((?r_state, ?r_regs), ?r_tl), ?r_inner).
+        simplify_invariant incr. logical_simplify.
+        subst. cbn. ssplit.
+        - auto.
+        - intros. discriminate.
+        - intros. auto.
+      }
+      eapply incr_invariant_preserved in Hinv as Hinv'; [|reflexivity].
+      unfold counter_related. exists (update_repr (c:=incr) (h2d, tt) repr).
+      rewrite surjective_pairing with (A:=counter_device) (B:=tl_d2h)
+                                      (p:=Semantics.step incr sL1 (h2d, tt)) in Hstep.
+      apply pair_equal_spec in Hstep. destruct Hstep as [Hstep1 Hstep2]. subst.
+      split; [| apply Hinv'; apply Hprec].
+      inversion Hrel; subst;
+        destruct_tl_h2d; destruct_tl_d2h; tlsimpl; subst;
+          cbn in sL1; destruct sL1 as ((?busy, (?done, (?regs, ?d2h))), (?s_tl, ?s_inner));
+            simplify_invariant incr; logical_simplify; subst;
+              cbn -[replace].
+      all: try (destruct x as [|[|[|]]]);
+        destruct (outstanding_h2d r_tl), d_ready;
+        try destruct (TLUL.a_opcode t =? Get)%N, (TLUL.a_opcode t =? PutFullData)%N;
         try (rewrite incrN_word_to_bv);
-        try (constructor; try lia; simpl; boolsimpl; ssplit; reflexivity).
-    - (* state_machine_read_to_device_read_or_later: *)
-      case TODO.
-      (*
-      cbn [counter_device device.state device.is_ready_state device.run1 device.addr_range_start
-           device.addr_range_pastend device.maxRespDelay] in *.
-      cbn [increment_wait_state_machine
-             state_machine.state
-             state_machine.register
-             state_machine.is_initial_state
-             state_machine.read_step
-             state_machine.write_step
-             state_machine.reg_addr
-             state_machine.isMMIOAddr] in *.
-      simpl in sL. destruct sL as ((istate & value & tl_d2h) & tlul_state).
-      destruct_tl_d2h. destruct_tlul_adapter_reg_state.
-      destruct H as [v [sH' [Hbytes H]]]. rewrite Hbytes.
-      tlsimpl.
-      destruct r; simp.
+        boolsimpl; constructor; try assumption.
+      all: destruct H6; subst; destruct r_regs; cbn in H |- *; assumption.
+    - (* state_machine_read_to_device_read: *)
+      (* simpler because device.maxRespDelay=1 *)
+      intros ? ? ? ? [v [sH'' Hex_read]] [repr Hrel].
+      cbn in Hex_read. logical_simplify. rewrite  H1.
+      unfold counter_related.
+      match goal with
+      | |- context [ device.runUntilResp ?x _ _ ] =>
+        remember x as h2d eqn:Eh2d; replace x with h2d
+      end.
+      assert (Hprec: precondition incr (h2d, tt) repr).
+      { destruct_tl_h2d. tlsimpl.
+        cbn in sL; destruct sL as ((?busy, (?done, (?regs, ?d2h))), (?s_tl, ?s_inner)).
+        destruct repr as (((?r_state, ?r_regs), ?r_tl), ?r_inner).
+        simplify_invariant incr. logical_simplify.
+        subst. cbn. ssplit; intros; auto.
+      }
+      pose (r_ := r). destruct r.
       + (* r=VALUE *)
-        destruct_tl_h2d.
-        cbn in *. subst.
-
-        destruct_consistent_states. subst.
-        destruct outstanding; cbn in H1|-*; fwd.
-
-
-          eexists _, _, _; ssplit; try reflexivity; cbn; rewrite Z_word_N by lia;
-            try (eapply IDLE_related; unfold consistent_states; ssplit; reflexivity);
-            try (apply N_to_word_word_to_N).
+        pose (sH_ := sH); destruct sH; cbn in H2; try (exfalso; assumption); logical_simplify; subst.
+        inversion H; subst.
+        eapply runUntilResp_big_step with (s:=sL) in Hprec
+          as [n [inputs [sL' [repr' [d2h [sL'' [HrunU [HmaxRespDelay [Einputs [EsL' [Erepr' [Hpostc' [Ed_valid Hinv'']]]]]]]]]]]]]; subst; auto.
+        exists d2h, sL'', IDLE.
+        ssplit.
+        3: cbn; ssplit; try reflexivity; [].
+        * assumption.
+        * eexists.
+          split; [|apply Hinv''].
+          simplify_invariant incr.
+          simplify_invariant Incr.inner.
+          simplify_invariant (tlul_adapter_reg (reg_count:=2)).
+          cbn in sL''; destruct sL'' as ((?busy, (?done, (?regs, ?d2h))), (?s_tl, ?s_inner)).
+          clear HrunU.
+          pose (n_:=n). destruct n as [|[|n]].
+          3: unfold device.maxRespDelay, counter_device in HmaxRespDelay; exfalso; lia.
+          all: cbn [repeat fold_left] in *.
+          -- destruct Hpostc' as [req' [h2d' [regs' [d2h' [io_re' [io_we' [io_address' [io_data' [io_mask' Hpostc']]]]]]]]].
+             logical_simplify.
+             cbn in H5.
+             destruct (outstanding_h2d r_tl) eqn:Houts.
+             ++ logical_simplify. rewrite Ed_valid in * |-. discriminate.
+             ++ cbn in H5. logical_simplify.
+                destruct_tl_d2h. tlsimpl. subst.
+                simplify_invariant incr.
+                cbn in sL; destruct sL as ((?busy, (?done, (?regs, ?d2h))), (?s_tl, ?s_inner)).
+                cbn in Hinv'' |- *.
+                rewrite Houts in Hinv'' |- *. cbn in Hinv''. logical_simplify.
+                cbn in *.
+                logical_simplify. subst.
+                rewrite Z_word_N in * by lia. cbn in *. logical_simplify. subst.
+                apply IDLE_related.
+          -- cbn in Hpostc'.
+             destruct (outstanding_h2d r_tl) eqn:Houts;
+             destruct Hpostc' as [req' [h2d' [regs' [d2h' [io_re' [io_we' [io_address' [io_data' [io_mask' Hpostc']]]]]]]]];
+             logical_simplify;
+             cbn in H5; rewrite Houts in H5; cbn in H5; logical_simplify; subst.
+             ++ destruct_tl_d2h. tlsimpl. subst.
+                simplify_invariant incr.
+                cbn in sL; destruct sL as ((?busy, (?done, (?regs, ?d2h))), (?s_tl, ?s_inner)).
+                cbn in Hinv'' |- *.
+                rewrite Houts in Hinv'' |- *. cbn in Hinv'' |- *. logical_simplify.
+                rewrite Houts. cbn.
+                rewrite Z_word_N in * by lia. cbn in *.
+                destruct H8; subst; apply IDLE_related.
+             ++ rewrite Ed_valid in * |-. discriminate.
+        * pose (n_:=n). destruct n as [|[|n]].
+          -- cbn [repeat fold_left] in *.
+             destruct Hpostc' as [req' [h2d' [regs' [d2h' [io_re' [io_we' [io_address' [io_data' [io_mask' Hpostc']]]]]]]]].
+             logical_simplify.
+             cbn in H5.
+             destruct (outstanding_h2d r_tl) eqn:Houts.
+             ++ logical_simplify. rewrite Ed_valid in * |-. discriminate.
+             ++ cbn in H5. logical_simplify.
+                destruct_tl_d2h. tlsimpl. subst.
+                simplify_invariant incr.
+                cbn in sL; destruct sL as ((?busy, (?done, (?regs, ?d2h))), (?s_tl, ?s_inner)).
+                cbn in sL''; destruct sL'' as ((?busy, (?done, (?regs, ?d2h))), (?s_tl, ?s_inner)).
+                cbn in Hinv''.
+                rewrite Houts in Hinv''. cbn in Hinv''. logical_simplify.
+                cbn in *.
+                logical_simplify. subst.
+                rewrite Z_word_N in * by lia. cbn in *. logical_simplify. subst.
+                rewrite H3. apply N_to_word_word_to_N.
+          -- cbn [repeat fold_left] in *.
+             cbn in Hpostc'.
+             destruct (outstanding_h2d r_tl) eqn:Houts;
+             destruct Hpostc' as [req' [h2d' [regs' [d2h' [io_re' [io_we' [io_address' [io_data' [io_mask' Hpostc']]]]]]]]];
+             logical_simplify;
+             cbn in H5; rewrite Houts in H5; cbn in H5; logical_simplify; subst.
+             ++ destruct_tl_d2h. tlsimpl. subst.
+                simplify_invariant incr.
+                cbn in sL; destruct sL as ((?busy, (?done, (?regs, ?d2h))), (?s_tl, ?s_inner)).
+                cbn in sL''; destruct sL'' as ((?busy, (?done, (?regs, ?d2h))), (?s_tl, ?s_inner)).
+                cbn in Hinv''.
+                rewrite Houts in Hinv''. cbn in Hinv''. logical_simplify.
+                rewrite Z_word_N in * by lia. cbn -[replace] in *.
+                destruct H8; subst; destruct r_regs; cbn in H3 |- *;
+                  rewrite H3; apply N_to_word_word_to_N.
+             ++ rewrite Ed_valid in * |-. discriminate.
+          -- unfold device.maxRespDelay, counter_device in HmaxRespDelay. exfalso. lia.
       + (* r=STATUS *)
-        destruct sH; [| |].
-        * (* sH=IDLE *)
-          inversion H0. subst.
-          destruct_consistent_states. subst. cbn.
-          repeat (rewrite Z_word_N by lia; cbn).
-          unfold status_value, STATUS_IDLE, N_to_word, word_to_N.
-          destruct outstanding; eexists _, _, _; ssplit; try reflexivity;
-              try (apply IDLE_related; simpl; ssplit; reflexivity);
-              try (simpl; unfold N_to_word; ZnWords).
-        * (* sH=BUSY *)
-          simpl.
-          unfold STATUS_ADDR, INCR_BASE_ADDR, N_to_word, word_to_N, status_value, STATUS_BUSY.
-          rewrite word.unsigned_of_Z. unfold word.wrap.
-          inversion H0; subst; [| |].
-          -- (* BUSY1_related *)
-            destruct outstanding; eexists _, _, _; simpl; [|].
-            ++ ssplit; try reflexivity; [|].
-               ** rewrite incrN_word_to_bv.
-                  apply BUSY_done_related; unfold consistent_states; ssplit; reflexivity.
-               ** right. eexists. ssplit; try reflexivity; [|].
-                  --- apply Nat.pred_inj; try lia. rewrite Nat.pred_succ. reflexivity.
-                  --- simpl. ZnWords.
-            ++ ssplit; try reflexivity; [|].
-               ** apply BUSY2_related. 1: shelve. unfold consistent_states. ssplit; reflexivity.
-               ** right. eexists. ssplit; try reflexivity; [|].
-                  --- apply Nat.pred_inj; try lia. rewrite Nat.pred_succ. reflexivity.
-                  --- simpl. ZnWords.
-                      Unshelve. lia.
-          -- (* BUSY2_related *)
-            destruct outstanding; eexists _, _, _; simpl; [|].
-            ++ ssplit; try reflexivity; [|].
-              ** rewrite incrN_word_to_bv.
-                 apply DONE_related; unfold consistent_states; ssplit; reflexivity.
-              ** left. simpl. ssplit; try reflexivity. ZnWords.
-            ++ ssplit; try reflexivity; [|].
-              ** rewrite incrN_word_to_bv.
-                 apply BUSY_done_related; unfold consistent_states; ssplit; reflexivity.
-              ** right. eexists. ssplit; try reflexivity; [|].
-                 --- apply Nat.pred_inj; try lia. rewrite Nat.pred_succ. reflexivity.
-                 --- simpl. ZnWords.
-          -- (* BUSY_done_related *)
-            (* the transition that was used to show that sH is not stuck was *)
-            (* a transition from BUSY to BUSY returning a busy flag, but *)
-            (* since the device already is in done state, it will return a *)
-            (* done flag in this transition, so the transition we use to *)
-            (* simulate what happened in the device is a BUSY-to-DONE *)
-            (* transition returning a done flag instead of a BUSY-to-BUSY *)
-            (* transition returning a busy flag. *)
-            destruct outstanding; eexists _, _, _; boolsimpl; simpl;
-              ssplit; try reflexivity;
-                try (apply DONE_related; unfold consistent_states; ssplit; reflexivity);
-                try (left; split; try reflexivity; simpl; ZnWords).
-        * (* sH=DONE *)
-          simpl.
-          unfold STATUS_ADDR, INCR_BASE_ADDR, N_to_word, word_to_N, status_value, STATUS_BUSY.
-          rewrite !word.unsigned_of_Z. unfold word.wrap.
-          inversion H0. subst.
-          destruct outstanding; eexists _, _, _; boolsimpl; simpl;
-            ssplit; try reflexivity;
-              try (eapply DONE_related; unfold consistent_states; ssplit; reflexivity);
-              try (simpl; ZnWords).
-      *)
-    - (* state_machine_write_to_device_write_or_later: *)
-      case TODO.
-      (*
-      destruct H as (sH' & ? & ?). subst.
-      unfold write_step in H1.
-      destruct r. 2: contradiction.
-      destruct sH; try contradiction. subst.
-      inversion H0. simpl in tl_d2h. simpl in tlul_state.
-      destruct_tl_d2h. destruct_tlul_adapter_reg_state. subst. cbn.
-      unfold word_to_N.
-      rewrite word.unsigned_of_Z_nowrap by (cbv; intuition discriminate).
-      destruct outstanding; boolsimpl; simpl;
-        eexists _, _, _; ssplit; try reflexivity; try assumption; apply BUSY1_related;
-          try lia;
-          try (unfold consistent_states; ssplit; reflexivity).
-      *)
+        eapply runUntilResp_big_step in Hprec as [n [inputs [sL' [repr' [d2h [sL'' [HrunU [HmaxRespDelay [Einputs [EsL' [Erepr' [Hpostc' [Ed_valid Hinv'']]]]]]]]]]]]]; subst; auto; [|eassumption].
+        inversion H; subst.
+        * do 3 eexists; ssplit.
+          -- rewrite HrunU; reflexivity.
+          -- eexists; split; [|eassumption];
+               destruct n as [|[|n]];
+               [| |unfold device.maxRespDelay, counter_device in HmaxRespDelay; exfalso; lia];
+               cbn [repeat fold_left] in *;
+               simplify_invariant incr;
+               cbn in sL; destruct sL as ((?busy, (?done, (?regs, ?d2h))), (?s_tl, ?s_inner));
+                 logical_simplify; subst;
+                   cbn; destruct (outstanding_h2d r_tl) eqn:Eouts;
+                     try (cbn; rewrite Eouts; cbn);
+                     apply IDLE_related.
+          -- cbn. ssplit; try reflexivity.
+             destruct n as [|[|n]];
+               [| |unfold device.maxRespDelay, counter_device in HmaxRespDelay; exfalso; lia];
+               cbn [repeat fold_left] in *; simplify_spec incr;
+                 simplify_spec (tlul_adapter_reg (reg_count:=2)).
+             ++ destruct Hpostc' as [req' [h2d' [regs' [d2h' [io_re' [io_we' [io_address' [io_data' [io_mask' Hpostc']]]]]]]]]; logical_simplify; cbn in H5;
+                  destruct (outstanding_h2d r_tl) eqn:Eouts;
+                  [logical_simplify; rewrite Ed_valid in *; discriminate|];
+                  cbn in H5; logical_simplify; rewrite H9.
+                unfold status_value, STATUS_IDLE, N_to_word, word_to_N.
+                simplify_invariant incr.
+                cbn in sL; destruct sL as ((?busy, (?done, (?regs, ?d2h))), (?s_tl, ?s_inner)).
+                logical_simplify.
+                replace (N.to_nat ((N.land (Z.to_N (word.unsigned (word.of_Z 16388))) 4 / 4) mod 1073741824)) with 1.
+                ** ZnWords.
+                ** ZnWords_pre. rewrite Zmod_small; [|lia].
+                   rewrite N.mod_small; cbn; lia.
+             ++ admit.
+        * admit.
+        * admit.
+        * admit.
+    - (* state_machine_write_to_device_write: *)
+      admit.
     - (* read_step_unique: *)
-      simpl in *. unfold read_step in *. simp.
+      intros. simpl in *. unfold read_step in *. simp.
       destruct v; destruct r; try contradiction; simp; try reflexivity.
       destruct Hp1; destruct H0p1; simp; try reflexivity;
         unfold status_value in *; exfalso; ZnWords.
     - (* write_step_unique: *)
-      simpl in *. unfold write_step in *. simp. subst. reflexivity.
+      intros. simpl in *. unfold write_step in *. simp. subst. reflexivity.
     - (* initial_state_unique: *)
-      simpl in *. subst. reflexivity.
+      intros. simpl in *. subst. reflexivity.
   Qed.
 End WithParameters.
